

$$\sinh x = \frac{e^x - e^{-x}}{2}$$

$$\cosh x = \frac{e^x + e^{-x}}{2}$$

1. A partial differential equation involves
  - a) 1 independent variable
  - b) 2 independent variables
  - c) 2 or more independent variables
  - d) None of these

Q Solve the Laplace equation  $\frac{\partial^2 u}{\partial x^2} + \frac{\partial^2 u}{\partial y^2} = 0$

Subject to the conditions

$$u(0, y) = u(l, y) = u(x, 0) = 0$$

$$\text{and } u(x, a) = \sin \frac{n\pi x}{l}$$

Sol The three possible solutions of

$$\frac{\partial^2 u}{\partial x^2} + \frac{\partial^2 u}{\partial y^2} = 0 \quad \text{--- (1) are :}$$

$$u = (C_1 e^{bx} + C_2 e^{-bx}) (C_3 \cos py + C_4 \sin py) \quad \text{--- (2)}$$

$$u = (C_5 \cos px + C_6 \sin px) (C_7 e^{py} + C_8 e^{-py}) \quad \text{--- (3)}$$

$$u = (C_9 x + C_{10}) (C_{11} y + C_{12}) \quad \text{--- (4)}$$

We have to solve ① which satisfies the following boundary conditions:

$$u(0, y) = 0 \text{ --- } \textcircled{5}$$

$$u(l, y) = 0 \text{ --- } \textcircled{6}$$

$$u(x, 0) = 0 \text{ --- } \textcircled{7}$$

$$u(x, a) = \sin \frac{n\pi x}{l} \text{ --- } \textcircled{8}$$

using (5) and (6) in (2),

$$u = (C_1 e^{px} + C_2 e^{-px}) (C_3 \cos py + C_4 \sin py) \quad \text{--- (2)}$$

$$u(0, y) = 0 \quad \text{--- (5)}$$

$$u(l, y) = 0 \quad \text{--- (6)}$$

using (5) in (2), we get

$$0 = (C_1 + C_2) (C_3 \cos py + C_4 \sin py)$$

$$\Rightarrow C_1 + C_2 = 0$$

using (6) in (2), we get

$$0 = (C_1 e^{pl} + C_2 e^{-pl}) (C_3 \cos py + C_4 \sin py)$$

$$\Rightarrow C_1 e^{pl} + C_2 e^{-pl} = 0$$

$$(c_1 + c_2) = 0 \quad \text{and} \quad c_1 e^{pl} + c_2 e^{-pl} = 0$$

On solving these equations, we get

$$c_1 = c_2 = 0$$

$$\therefore c_1 = -c_2 \quad \text{and} \quad c_1 e^{pl} - c_1 e^{-pl} = 0$$

$$\Rightarrow c_1 [e^{pl} - e^{-pl}] = 0 \Rightarrow c_1 = 0$$
$$\Rightarrow c_2 = 0$$

which leads to trivial solution.

Now using (5) and (6) in (4)

where (4) is  $\rightarrow$

$$u = (c_9 x + c_{10}) (c_{11} y + c_{12}) \quad \text{--- (4)}$$

$$u(0, y) = 0 \quad \text{--- (5)}$$

$$u(1, y) = 0 \quad \text{--- (6)}$$

$$\therefore (4) \Rightarrow (c_{10}) (c_{11} y + c_{12}) = 0$$

$$\Rightarrow c_{10} = 0$$



$$\therefore \textcircled{4} \Rightarrow u = c_9 x (c_{11} y + c_{12})$$

$$\text{and } u(c, y) = 0$$

$$\Rightarrow c_9 l (c_{11} y + c_{12}) = 0$$

$$\Rightarrow c_9 = 0$$

$$\Rightarrow u = 0$$

which is a trivial solution.

Hence the suitable solution for the present problem is solution  $\textcircled{3}$ .

Using (5) in (3) we get

Here (5) is  $u(0, y) = 0$

(3) is  $u = (C_5 \cos px + C_6 \sin px) (C_7 e^{py} + C_8 e^{-py})$

Now  $u(0, y) = 0$

$$\Rightarrow C_5 (C_7 e^{py} + C_8 e^{-py}) = 0$$

$$\Rightarrow \boxed{C_5 = 0}$$

$$\therefore \textcircled{3} \Rightarrow u = c_6 \sin px \left( c_7 e^{py} + c_8 e^{-py} \right) \quad \text{---} \textcircled{9}$$

Using  $\textcircled{6}$ , i.e.  $u(l, y) = 0$

$$\textcircled{9} \Rightarrow c_6 \sin pl \left( c_7 e^{py} + c_8 e^{-py} \right) = 0$$

$$\Rightarrow c_6 = 0 \quad \text{or} \quad \sin pl = 0$$

If we take  $c_6 = 0$ , we get trivial solution.

$$\text{Thus } \sin pl = 0$$

$$\Rightarrow pl = n\pi$$

$$\Rightarrow p = \frac{n\pi}{l}, \quad n \rightarrow \text{integer}$$

$\therefore$  (9) becomes.

$$u = C_6 \sin \frac{n\pi}{l} x \left[ C_7 e^{\frac{n\pi}{l} y} + C_8 e^{-\frac{n\pi}{l} y} \right] \quad \text{--- (10)}$$

using (7) i.e.  $u(x, 0) = 0$

$$\textcircled{10} \Rightarrow C_6 \sin \frac{n\pi}{\ell} x [C_7 + C_8] = 0$$

$$\Rightarrow C_7 + C_8 = 0$$

$$\because C_6 \neq 0 \text{ since } C_6 = 0$$

$$\Rightarrow u = 0 \text{ (trivial sol)}$$

$$\Rightarrow C_8 = -C_7$$

$$\therefore u(x, y) = C_6 \sin \frac{n\pi}{\ell} x \left[ C_7 e^{\frac{n\pi y}{\ell}} - C_7 e^{-\frac{n\pi y}{\ell}} \right]$$

$$= C_6 C_7 \sin \frac{n\pi}{\ell} x \left[ e^{\frac{n\pi y}{\ell}} - e^{-\frac{n\pi y}{\ell}} \right]$$

$$u(x, y) = b_n \sin \frac{n\pi x}{l} \left[ e^{\frac{n\pi y}{l}} - e^{-\frac{n\pi y}{l}} \right]$$

————— (11)

Using condition (8), i.e.  $u(x, a) = \sin \frac{n\pi x}{l}$

$$(11) \Rightarrow b_n \sin \frac{n\pi x}{l} \left[ e^{\frac{n\pi a}{l}} - e^{-\frac{n\pi a}{l}} \right] = \sin \frac{n\pi x}{l}$$

$$\Rightarrow b_n \left[ e^{\frac{n\pi a}{l}} - e^{-\frac{n\pi a}{l}} \right] = 1$$



$$\Rightarrow b_n = \frac{1}{e^{\frac{n\pi a}{c}} - e^{-\frac{n\pi a}{c}}}$$

$\therefore$  required solution is

$$u(x, y) = \frac{\left[ e^{\frac{n\pi y}{c}} - e^{-\frac{n\pi y}{c}} \right]}{\left[ e^{\frac{n\pi a}{c}} - e^{-\frac{n\pi a}{c}} \right]} \sin \frac{n\pi x}{c}$$

$$u(x, y) = \frac{\sinh\left(\frac{n\pi y}{a}\right) \sin \frac{n\pi x}{a}}{\sinh\left(\frac{n\pi a}{a}\right)}$$

which is the required solution.